compiler/eval/compilerComputeLib.sml
@@ -176,6 +176,8 @@ val add_compiler_compset = computeLib.extend_compset
     ,closLangTheory.pure_op_def
       (* ---- pat_to_clos ---- *)
     ,pat_to_closTheory.compile_def
+    ,pat_to_closTheory.CopyByteStr_def
+    ,pat_to_closTheory.CopyByteAw8_def
     ,pat_to_closTheory.vector_tag_def
     ,pat_to_closTheory.compile_def
       (*,pat_to_closTheory.pat_tag_shift_def*)
